phase splitting the lemmas.

MirrorCharge!/src/OrderedCanceller.v
@@ -133,18 +133,23 @@ Section ordered_cancel.
   Variable PureOp_SL : @Pure.PureOp (typD ts nil tySL).
   Variable Pure_SL : Pure.Pure PureOp_SL.
   Hypothesis Pure_ltrue : Pure.pure ltrue.
+  Hypothesis Pure_land : forall a b, Pure.pure a -> Pure.pure b -> Pure.pure (a //\\ b).
 
-  Fixpoint well_formed_Conjuncts (ls : Conjuncts) : Prop :=
-    match ls with
-      | Emp => True
-      | Tru => True
-      | Pure p ls =>
-        match exprD us vs p tySL with
-          | None => False
-          | Some p => Pure.pure p
-        end /\ well_formed_Conjuncts ls
-      | Impure _ _ ls => well_formed_Conjuncts ls
-    end.
+  Section well_formed_Conjuncts.
+    Variable us' vs' : EnvI.env (typD ts).
+
+    Fixpoint well_formed_Conjuncts (ls : Conjuncts) : Prop :=
+      match ls with
+        | Emp => True
+        | Tru => True
+        | Pure p ls =>
+          match exprD us' vs' p tySL with
+            | None => False
+            | Some p => Pure.pure p
+          end /\ well_formed_Conjuncts ls
+        | Impure _ _ ls => well_formed_Conjuncts ls
+      end.
+  End well_formed_Conjuncts.
 
   Fixpoint Conjuncts_to_expr (ls : Conjuncts) : expr func :=
     match ls with
@@ -155,7 +160,6 @@ Section ordered_cancel.
       | Impure f xs ls =>
         SSL.(e_star) (apps f xs) (Conjuncts_to_expr ls)
     end.
-
 
   Definition sentails : env (typD ts) -> env (typD ts) -> expr func -> expr func -> Prop :=
     @Sem_equiv ts func _ tySL lentails.
@@ -168,7 +172,7 @@ Section ordered_cancel.
         exprD' us tvs (iterated_base SSL.(e_emp) SSL.(e_star) b) tySL = Some bV /\
         (forall vs, ((x vs) -|- sepSP (aV vs) (bV vs))).
   Proof.
-    clear Pure_SL PureOp_SL Pure_ltrue.
+    clear Pure_SL PureOp_SL Pure_ltrue Pure_land.
     unfold iterated_base. simpl.
     intros.
     destruct (iterated (e_star SSL) b).
@@ -185,7 +189,7 @@ Section ordered_cancel.
       exprD' us tvs a tySL = None \/
       exprD' us tvs (iterated_base SSL.(e_emp) SSL.(e_star) b) tySL = None.
   Proof.
-    clear Pure_SL PureOp_SL Pure_ltrue.
+    clear Pure_SL PureOp_SL Pure_ltrue Pure_land.
     unfold iterated_base. simpl.
     intros.
     destruct (iterated (e_star SSL) b); auto.
@@ -198,7 +202,6 @@ Section ordered_cancel.
       destruct (SSLO.(e_empOk) us0 tvs). intuition. congruence. }
   Qed.
 
-
   Lemma exprD'_iterated_base_app_Some
   : forall us tvs a b x,
       exprD' us tvs (iterated_base SSL.(e_emp) SSL.(e_star) (a ++ b)) tySL = Some x ->
@@ -207,7 +210,7 @@ Section ordered_cancel.
         exprD' us tvs (iterated_base SSL.(e_emp) SSL.(e_star) b) tySL = Some bV /\
         (forall vs, ((x vs) -|- sepSP (aV vs) (bV vs))).
   Proof.
-    clear Pure_SL PureOp_SL doUnifySepLogOk Pure_ltrue.
+    clear Pure_SL PureOp_SL doUnifySepLogOk Pure_ltrue Pure_land.
     induction a; simpl; intros.
     { destruct (SSLO.(e_empOk) us0 tvs) as [ ? [ ? ? ] ].
       exists x0. exists x.
@@ -236,7 +239,7 @@ Section ordered_cancel.
       exprD' us tvs (iterated_base SSL.(e_emp) SSL.(e_star) a) tySL = None \/
       exprD' us tvs (iterated_base SSL.(e_emp) SSL.(e_star) b) tySL = None.
   Proof.
-    clear Pure_SL PureOp_SL doUnifySepLogOk Pure_ltrue.
+    clear Pure_SL PureOp_SL doUnifySepLogOk Pure_ltrue Pure_land.
     induction a; simpl; intros.
     { intuition.
       unfold iterated_base in H0. simpl in *.
@@ -246,27 +249,180 @@ Section ordered_cancel.
       rewrite IHa. split; tauto. }
   Qed.
 
+  Lemma cancelOk_lem'
+  : forall us tvs rhs lhs rem s lhs' rhs' s',
+      cancel rhs lhs rem s = (lhs',rhs',s') ->
+      match
+          exprD' us tvs (conjunctives_to_expr_star SSL lhs) tySL
+        , exprD' us tvs (SSL.(e_star) (conjunctives_to_expr_star SSL rem)
+                                      (Conjuncts_to_expr rhs)) tySL
+      with
+        | Some l , Some r =>
+          match
+              exprD' us tvs (conjunctives_to_expr_star SSL lhs') tySL
+            , exprD' us tvs (conjunctives_to_expr_star SSL rhs') tySL
+          with
+            | Some l' , Some r' =>
+              forall vs,
+                well_formed _ _ _ lhs us (join_env vs) ->
+                well_formed_Conjuncts us (join_env vs) rhs ->
+                well_formed _ _ _ rem us (join_env vs) ->
+                   well_formed _ _ _ lhs' us (join_env vs)
+                /\ well_formed _ _ _ rhs' us (join_env vs)
+                /\ (substD us (join_env vs) s' ->
+                    (l' vs |-- r' vs) ->
+                    (l vs |-- r vs) /\ substD us (join_env vs) s)
+            | _ , _ => False
+          end
+        | _ , _ => True
+      end.
+  Proof.
+    induction rhs; intros; forward.
+    { repeat go_crazy SSL SSLO.
+      admit. }
+    { repeat go_crazy SSL SSLO.
+      simpl in H.
+      consider (findWithRest
+          (fun x : expr func * list (expr func) =>
+           doUnifySepLog s (apps f xs) (apps (fst x) (snd x)))
+          (spatial lhs) nil); intros.
+      { destruct p. destruct p.
+        eapply IHrhs in H4; clear IHrhs.
+        consider (exprD' us0 tvs
+           (conjunctives_to_expr_star SSL
+              {|
+              spatial := l;
+              star_true := star_true lhs;
+              pure := pure lhs |}) tySL); intros.
+        { consider (exprD' us0 tvs
+           (e_star SSL (conjunctives_to_expr_star SSL rem)
+              (Conjuncts_to_expr rhs)) tySL); intros.
+          { forward. repeat go_crazy SSL SSLO.
+            inv_all; subst.
+            admit. }
+          { exfalso. simpl in H2.
+            repeat (go_crazy SSL SSLO; try congruence). } }
+        { exfalso.
+          simpl in *. admit. } }
+      { eapply IHrhs in H4; clear IHrhs. clear H.
+        unfold conjunctives_to_expr_star in *; simpl in *.
+        progress forward.
+        inv_all; subst.
+        generalize dependent (e_star SSL
+                         (iterated_base (e_emp SSL) 
+                            (e_star SSL)
+                            (map
+                               (fun x : expr func * list (expr func) =>
+                                apps (fst x) (snd x)) 
+                               (spatial rhs')))
+                         (if star_true rhs' then e_true SSL else e_emp SSL)).
+        generalize dependent (e_star SSL
+             (iterated_base (e_emp SSL) (e_star SSL)
+                (map
+                   (fun x1 : expr func * list (expr func) =>
+                    apps (fst x1) (snd x1)) (spatial lhs')))
+             (if star_true lhs' then e_true SSL else e_emp SSL)).
+        intros.
+        repeat go_crazy SSL SSLO.
+        consider (exprD' us0 tvs
+           (e_star SSL
+              (e_star SSL
+                 (iterated_base (e_emp SSL) (e_star SSL)
+                    (map (e_and SSL (e_emp SSL)) (pure rem)))
+                 (e_star SSL
+                    (iterated_base (e_emp SSL) (e_star SSL)
+                       (apps f xs
+                        :: map
+                             (fun x : expr func * list (expr func) =>
+                              apps (fst x) (snd x)) 
+                             (spatial rem)))
+                    (if star_true rem then e_true SSL else e_emp SSL)))
+              (Conjuncts_to_expr rhs)) tySL); intros.
+        { forward. admit. }
+        { exfalso.
+          repeat go_crazy SSL SSLO.
+          eapply exprD'_iterated_base_cons_None in H4.
+          destruct H4; congruence. } } }
+    { simpl in H. inv_all; subst.
+      simpl in *.
+      destruct (SSLO.(e_empOk) us0 tvs) as [ ? [ ? ? ] ].
+      repeat go_crazy SSL SSLO.
+      inv_all; subst.
+      intros.
+      split; auto. split; auto. intros. split; auto.
+      rewrite H8.
+      rewrite H4. rewrite H2.
+      rewrite empSPR; eauto. }
+    { simpl in H. inv_all; subst.
+      simpl in *.
+      destruct (SSLO.(e_empOk) us0 tvs) as [ ? [ ? ? ] ].
+      repeat go_crazy SSL SSLO.
+      unfold conjunctives_to_expr_star. simpl.
+      unfold conjunctives_to_expr_star in H1.
+      generalize dependent (iterated_base (e_emp SSL) (e_star SSL)
+               (map (e_and SSL (e_emp SSL)) (pure rem))).
+      generalize dependent (iterated_base (e_emp SSL) (e_star SSL)
+                (map
+                   (fun x2 : expr func * list (expr func) =>
+                    apps (fst x2) (snd x2)) (spatial rem))).
+      intros.
+      repeat go_crazy SSL SSLO.
+      consider (exprD' us0 tvs (e_star SSL e0 (e_star SSL e (e_true SSL))) tySL); intros.
+      { split; auto. split; auto.
+        intros; split; auto.
+        rewrite H14; clear H14.
+        repeat go_crazy SSL SSLO.
+        inv_all; subst.
+        rewrite H4; clear H4.
+        rewrite H6; clear H6.
+        rewrite H15; clear H15.
+        rewrite H17; clear H17.
+        rewrite H8; clear H8.
+        destruct (SSLO.(e_trueOk) us0 tvs) as [ ? [ ? ? ] ].
+        rewrite H3 in *. inv_all; subst.
+        rewrite H6.
+        destruct (star_true rem); rewrite H7 in *; inv_all; subst.
+        { rewrite H6.
+          repeat rewrite sepSPA.
+          rewrite ltrue_sep; eauto. reflexivity. }
+        { rewrite H2. rewrite empSPR; eauto.
+          rewrite sepSPA; eauto. reflexivity. } }
+      { repeat (go_crazy SSL SSLO; try congruence). } }
+  Qed.
+
+(*
   Lemma cancelOk_lem
   : forall rhs lhs rem s lhs' rhs' s',
       cancel rhs lhs rem s = (lhs',rhs',s') ->
       well_formed _ _ _ lhs us vs ->
       well_formed_Conjuncts rhs ->
       well_formed _ _ _ rem us vs ->
-      sentails us vs (conjunctives_to_expr_star SSL lhs')
-                     (conjunctives_to_expr_star SSL rhs') ->
+      substD us vs s' ->
+      match exprD us vs (conjunctives_to_expr_star SSL lhs') tySL
+          , exprD us vs (conjunctives_to_expr_star SSL rhs') tySL
+      with
+        | Some l , Some r =>
+          l |-- r
+        | _ , _ => True
+      end ->
       match exprD us vs (conjunctives_to_expr_star SSL lhs) tySL
           , exprD us vs (SSL.(e_star) (conjunctives_to_expr_star SSL rem)
                                       (Conjuncts_to_expr rhs)) tySL
       with
-        | Some l , Some r => l |-- r
+        | Some l , Some r =>
+             l |-- r
+          /\ well_formed _ _ _ lhs' us vs
+          /\ well_formed _ _ _ rhs' us vs
+          /\ substD us vs s
         | _ , _ => True
       end.
   Proof.
+  (*
     unfold sentails.
     induction rhs; intros.
     { simpl in H.
       specialize (IHrhs _ _ _ _ _ _ H H0).
-      simpl in H1. forward. destruct H4.
+      simpl in H1. forward. destruct H5.
       (** TODO: this is about provability and it isn't implemented yet **)
       admit. }
     { simpl in H.
@@ -287,7 +443,8 @@ Section ordered_cancel.
         assert (well_formed_Conjuncts rhs).
         { simpl in *; auto. }
         assert (well_formed RSym_func tySL PureOp_SL rem us vs) by auto.
-        specialize (IHrhs _ _ _ _ _ _ H4 H11 H12 H13 H3); clear H11 H12 H13 H3 H4.
+        admit. (*
+        specialize (IHrhs _ _ _ _ _ _ H5 H12 H13 H14); clear H11 H12 H13 H3 H4.
         repeat go_crazy SSL SSLO.
         inv_all; subst.
         eapply findWithRest_spec in H.
@@ -332,7 +489,17 @@ Section ordered_cancel.
           assert (x17 h ** (x19 h ** x11 h ** x14 h ** x22 h) |--
                   x2 h ** (x7 h ** x9 h ** x10 h ** x6 h)).
           { apply scME.
-            { admit. }
+            { eapply doUnifySepLogOk in H.
+              { rewrite H7 in *.
+                rewrite H20 in *.
+                destruct H.
+                inv_all; subst.
+                rewrite H. reflexivity. }
+              { admit. }
+              { admit. }
+              { admit. }
+              { 
+ }
             { etransitivity. etransitivity.
               2: eapply IHrhs.
               clear IHrhs. Cases.rewrite_all_goal.
@@ -354,7 +521,7 @@ Section ordered_cancel.
           repeat go_crazy SSL SSLO.
           rewrite map_app in H24.
           apply exprD'_iterated_base_app_None in H24.
-          destruct H24; congruence. } }
+          destruct H24; congruence. } *) }
       { (** findWithRest returns None **)
         unfold Sem_equiv in *.
         forward.
@@ -365,7 +532,8 @@ Section ordered_cancel.
                               spatial := spatial rem;
                               star_true := star_true rem;
                               pure := pure rem |} us vs) by auto.
-        specialize (IHrhs _ _ _ _ _ _ H4 H7 H8 H9 H3); clear H4 H3 H7 H8 H9.
+        specialize (IHrhs _ _ _ _ _ _ H5 H8 H9 H10); clear H5 H8 H9 H10.
+        admit. (*
         rewrite H5 in *. simpl in *. clear H.
         consider (exprD us vs
               (e_star SSL
@@ -401,11 +569,11 @@ Section ordered_cancel.
           inv_all; subst.
           repeat (go_crazy SSL SSLO; try congruence).
           eapply exprD'_iterated_base_cons_None in H.
-          destruct H; congruence. } } }
+          destruct H; congruence. } *) } }
     { simpl in *.
       inv_all; subst.
       forward.
-      red in H3.
+      red in H4.
       unfold exprD in *.
       destruct (split_env vs).
       forward. inv_all; subst.
@@ -417,12 +585,12 @@ Section ordered_cancel.
       reflexivity. }
     { simpl in *.
       inv_all; subst.
-      red in H3. unfold exprD in *. forward.
+      red in H4. unfold exprD in *. forward.
       inv_all; subst.
       destruct (SSLO.(e_trueOk) us x) as [ ? [ ? ? ] ].
       repeat go_crazy SSL SSLO.
       inv_all; subst.
-      rewrite H4; clear H4 H3.
+      rewrite H5; clear H5 H4.
       destruct rem.
       unfold conjunctives_to_expr_star in *. simpl in *.
       repeat go_crazy SSL SSLO.
@@ -432,22 +600,33 @@ Section ordered_cancel.
       apply scME; try reflexivity.
       apply scME; try reflexivity.
       destruct star_true.
-      { rewrite H8 in *. inv_all; subst.
+      { rewrite H9 in *. inv_all; subst.
         Cases.rewrite_all.
         eapply ltrue_sep; eauto with typeclass_instances. }
       { destruct (SSLO.(e_empOk) us x).
-        rewrite H8 in *.
-        destruct H3.
+        rewrite H9 in *.
+        destruct H4.
         inv_all; subst.
-        rewrite H4. rewrite empSPL. apply ltrueR. } }
+        rewrite H5. rewrite empSPL. apply ltrueR. } }
   Qed.
+*)
+  Admitted.
+*)
 
   Variable order : conjunctives func -> Conjuncts.
-(*
-  Hypothesis orderOk : forall c us vs,
-    well_formed _ c us vs ->
-    sentails (Conjuncts_to_expr (order c)) (conjunctives_to_expr c).
-*)
+  Hypothesis orderOk
+  : forall c us tvs,
+      match exprD' us tvs (conjunctives_to_expr_star SSL c) tySL
+          , exprD' us tvs (Conjuncts_to_expr (order c)) tySL
+      with
+        | Some l , Some r =>
+          forall vs,
+            well_formed _ _ _ c us (join_env vs) ->
+            ((l vs -|- r vs) /\
+             well_formed_Conjuncts us (join_env vs) (order c))
+        | None , None => True
+        | _ , _ => False
+      end.
 
   Definition ordered_cancel (lhs rhs : conjunctives func) (s : subst)
   : conjunctives func * conjunctives func * subst :=
@@ -455,22 +634,149 @@ Section ordered_cancel.
     let empty := {| spatial := nil ; pure := nil ; star_true := false |} in
     cancel ordered lhs empty s.
 
+  Theorem ordered_cancelOk
+  : forall us tvs lhs rhs s lhs' rhs' s',
+      ordered_cancel lhs rhs s = (lhs', rhs', s') ->
+      match
+          exprD' us tvs (conjunctives_to_expr SSL lhs) tySL
+        , exprD' us tvs (conjunctives_to_expr SSL rhs) tySL
+      with
+        | Some l , Some r =>
+          match
+              exprD' us tvs (conjunctives_to_expr SSL lhs') tySL
+            , exprD' us tvs (conjunctives_to_expr SSL rhs') tySL
+          with
+            | Some l' , Some r' =>
+              forall vs', let vs := join_env vs' in
+              
+              well_formed _ _ _ lhs us vs ->
+              well_formed _ _ _ rhs us vs ->
+              substD us vs s' ->
+                  well_formed _ _ _ lhs' us vs
+               /\ well_formed _ _ _ rhs' us vs
+               /\ ((l' vs' |-- r' vs') -> l vs' |-- r vs')
+            | _ , _ => False
+          end
+        | _ , _ => True
+      end.
+  Proof.
+    intros.
+    unfold ordered_cancel in H.
+    eapply cancelOk_lem' with (us := us0) (tvs := tvs) in H.
+    forward.
+    generalize (@conjunctives_to_expr_conjunctives_to_expr_star_iff _ _ _ _ _ SSL _ tvs us0 lhs).
+    generalize (@conjunctives_to_expr_conjunctives_to_expr_star_iff _ _ _ _ _ SSL _ tvs us0 rhs).
+    rewrite H0. rewrite H1.
+    specialize (orderOk rhs us0 tvs).
+    intros; forward.
+    match type of H3 with
+      | match ?X with _ => _ end =>
+        consider X; intros
+    end.
+    { forward.
+      unfold conjunctives_to_expr_star in H3; simpl in H3.
+      unfold iterated_base in H3; simpl in H3.
+      repeat go_crazy SSL SSLO.
+      inv_all; subst.
+      generalize (@conjunctives_to_expr_conjunctives_to_expr_star_iff _ _ _ _ _ SSL _ tvs us0 lhs').
+      generalize (@conjunctives_to_expr_conjunctives_to_expr_star_iff _ _ _ _ _ SSL _ tvs us0 rhs').
+      Cases.rewrite_all_goal.
+      intros; forward.
+      destruct (orderOk _ H18); clear orderOk.
+      assert (well_formed RSym_func tySL PureOp_SL
+         {| spatial := nil; star_true := false; pure := nil |} us0
+         (join_env vs')) by constructor.
+      specialize (H9 _ H17 H21 H22).
+      destruct H9 as [ ? [ ? ? ] ].
+      split; auto.
+      split; auto.
+      intro.
+      assert (t5 vs' |-- t6 vs').
+      { clear H24.
+        rewrite <- H14 by auto; clear H14.
+        rewrite <- H16 by auto; clear H16.
+        assumption. }
+      specialize (H24 H19 H26).
+      rewrite H5 by auto; clear H5.
+      rewrite H4 by auto; clear H4.
+      rewrite H20; clear H20.
+      destruct H24.
+      rewrite H4; clear H4.
+      rewrite H11; clear H11.
+      rewrite H13; clear H13.
+      rewrite H15; clear H15.
+      destruct (SSLO.(e_empOk) us0 tvs) as [ ? [ ? ? ] ].
+      rewrite H4 in *. inv_all; subst.
+      repeat rewrite H11.
+      repeat rewrite empSPL. reflexivity. }
+    { exfalso.
+      unfold conjunctives_to_expr_star in H3; simpl in H3.
+      unfold iterated_base in H3; simpl in H3.
+      destruct (SSLO.(e_empOk) us0 tvs).
+      destruct (SSLO.(e_trueOk) us0 tvs).
+      destruct H7; destruct H8.
+      repeat (go_crazy SSL SSLO; try congruence). }
+  Qed.
+
 End ordered_cancel.
 
 (** The simplest ordering heuristic just uses the order that they occur in the
  ** map without looking at unification variables.
  **)
 Section simple_ordering.
-  Variable typ : Type.
-  Variable typD : list Type -> typ -> Type.
-  Variable RType_typ : RType typD.
+  Variable ts : types.
   Variable func : Type.
-  Variable RSym_func : RSym typD func.
+  Variable RSym_func : RSym (typD ts) func.
 
-  Definition order_conjunctives (c : conjunctives func) : Conjuncts func :=
+  Variable tySL : typ.
+  Variable ILogicOps_SL : ILogicOps (typD ts nil tySL).
+  Variable BILOperators_SL : BILOperators (typD ts nil tySL).
+  Hypothesis ILogic_SL : @ILogic _ ILogicOps_SL.
+  Hypothesis BILogic_SL : @BILogic _ ILogicOps_SL BILOperators_SL.
+
+
+
+  Definition simple_order (c : conjunctives func) : Conjuncts func :=
     List.fold_right (fun x acc => Impure (fst x) (snd x) acc)
                     (List.fold_right (fun x acc => Pure x acc)
                                      (if c.(star_true) then Tru _ else Emp _)
                                      c.(pure))
                     c.(spatial).
+
+  Variable SSL : SynSepLog func.
+  Variable SSLO : SynSepLogOk _ _ _ _ SSL.
+
+  Variable PureOp_SL : @Pure.PureOp (typD ts nil tySL).
+  Variable Pure_SL : Pure.Pure PureOp_SL.
+  Hypothesis Pure_ltrue : Pure.pure ltrue.
+  Hypothesis Pure_land : forall a b, Pure.pure a -> Pure.pure b -> Pure.pure (a //\\ b).
+
+
+  Theorem simple_orderOk
+  : forall c us tvs,
+      match exprD' us tvs (conjunctives_to_expr_star SSL c) tySL
+          , exprD' us tvs (Conjuncts_to_expr SSL (simple_order c)) tySL
+      with
+        | Some l , Some r =>
+          forall vs,
+            well_formed _ _ _ c us (join_env vs) ->
+            ((l vs -|- r vs) /\
+             well_formed_Conjuncts _ tySL _ us (join_env vs) (simple_order c))
+        | None , None => True
+        | _ , _ => False
+      end.
+  Proof.
+    intros; destruct c; simpl.
+    unfold conjunctives_to_expr_star, simple_order; simpl.
+    match goal with
+      | |- match ?X with _ => _ end =>
+        consider X; intros
+    end.
+    { admit. }
+    { forward.
+(*      repeat go_crazy SSL SSLO. *)
+      admit. }
+  Qed.
+
+
 End simple_ordering.
