MirrorCharge!/src/SynSepLog.v
@@ -72,7 +72,7 @@ Section syn_sep_log.
                      exprD' us tvs x SL = Some valx /\
                      exprD' us tvs y SL = Some valy /\
                      forall vs, val vs -|- valx vs //\\ valy vs
-    }.
+  }.
 
   Variable SSLO : SynSepLogOk.
 
@@ -89,7 +89,8 @@ Section syn_sep_log.
              | H : _ /\ _ |- _ => destruct H
            end.
 
-  Lemma e_andOk_None1
+  (** Primed versions **)
+  Lemma exprD'_e_andOk_None1
   : forall us tvs x y,
       exprD' us tvs x SL = None ->
       exprD' us tvs (SSL.(e_and) x y) SL = None.
@@ -100,7 +101,7 @@ Section syn_sep_log.
     eapply e_andValid in H0; eauto. forward_ex_and. congruence.
   Qed.
 
-  Lemma e_andOk_None2
+  Lemma exprD'_e_andOk_None2
   : forall us tvs x y,
       exprD' us tvs y SL = None ->
       exprD' us tvs (SSL.(e_and) x y) SL = None.
@@ -111,7 +112,7 @@ Section syn_sep_log.
     eapply e_andValid in H0; eauto. forward_ex_and. congruence.
   Qed.
 
-  Lemma e_starOk_None1
+  Lemma exprD'_e_starOk_None1
   : forall us tvs x y,
       exprD' us tvs x SL = None ->
       exprD' us tvs (SSL.(e_star) x y) SL = None.
@@ -122,7 +123,7 @@ Section syn_sep_log.
     eapply e_starValid in H0; eauto. forward_ex_and. congruence.
   Qed.
 
-  Lemma e_starOk_None2
+  Lemma exprD'_e_starOk_None2
   : forall us tvs x y,
       exprD' us tvs y SL = None ->
       exprD' us tvs (SSL.(e_star) x y) SL = None.
@@ -132,16 +133,6 @@ Section syn_sep_log.
     exfalso.
     eapply e_starValid in H0; eauto. forward_ex_and. congruence.
   Qed.
-
-  Definition Sem_ext (t : typ) (P : typD ts nil t -> Prop) (Q : Prop)
-  : expr sym -> Prop :=
-    fun e =>
-      forall us tvs,
-        match exprD' us tvs e t with
-          | Some val =>
-            forall vs, P (val vs)
-          | None => Q
-        end.
 
   Lemma exprD'_e_and_None
   : forall us tvs a b,
@@ -167,6 +158,169 @@ Section syn_sep_log.
     exfalso.
     destruct (@e_starOk SSLO _ _ _ _ _ _ H0 H1).
     intuition; congruence.
+  Qed.
+
+  (** Unprimed versions **)
+  Lemma exprD_e_andOk_None1
+  : forall us vs x y,
+      exprD us vs x SL = None ->
+      exprD us vs (SSL.(e_and) x y) SL = None.
+  Proof.
+    intros.
+    consider (exprD us vs (SSL.(e_and) x y) SL); auto; intros.
+    exfalso.
+    unfold exprD in *. destruct (split_env vs).
+    forward.
+    eapply e_andValid in H0; eauto. forward_ex_and. congruence.
+  Qed.
+
+  Lemma exprD_e_andOk_None2
+  : forall us vs x y,
+      exprD us vs y SL = None ->
+      exprD us vs (SSL.(e_and) x y) SL = None.
+  Proof.
+    intros.
+    consider (exprD us vs (SSL.(e_and) x y) SL); auto; intros.
+    exfalso.
+    unfold exprD in *. destruct (split_env vs).
+    forward.
+    eapply e_andValid in H0; eauto. forward_ex_and. congruence.
+  Qed.
+
+  Lemma exprD_e_starOk_None1
+  : forall us vs x y,
+      exprD us vs x SL = None ->
+      exprD us vs (SSL.(e_star) x y) SL = None.
+  Proof.
+    intros.
+    consider (exprD us vs (SSL.(e_star) x y) SL); auto; intros.
+    exfalso.
+    unfold exprD in *. destruct (split_env vs).
+    forward.
+    eapply e_starValid in H0; eauto. forward_ex_and. congruence.
+  Qed.
+
+  Lemma exprD_e_starOk_None2
+  : forall us vs x y,
+      exprD us vs y SL = None ->
+      exprD us vs (SSL.(e_star) x y) SL = None.
+  Proof.
+    intros.
+    consider (exprD us vs (SSL.(e_star) x y) SL); auto; intros.
+    exfalso.
+    unfold exprD in *. destruct (split_env vs).
+    forward.
+    eapply e_starValid in H0; eauto. forward_ex_and. congruence.
+  Qed.
+
+  Lemma exprD_e_and_None
+  : forall us vs a b,
+      exprD us vs (SSL.(e_and) a b) SL = None ->
+      exprD us vs a SL = None \/ exprD us vs b SL = None.
+  Proof.
+    intros.
+    consider (exprD us vs a SL); intros; auto.
+    consider (exprD us vs b SL); intros; auto.
+    exfalso.
+    unfold exprD in *. destruct (split_env vs).
+    forward.
+    destruct (@e_andOk SSLO _ _ _ _ _ _ H0 H1).
+    intuition; congruence.
+  Qed.
+
+  Lemma exprD_e_star_None
+  : forall us vs a b,
+      exprD us vs (SSL.(e_star) a b) SL = None ->
+      exprD us vs a SL = None \/ exprD us vs b SL = None.
+  Proof.
+    intros.
+    consider (exprD us vs a SL); intros; auto.
+    consider (exprD us vs b SL); intros; auto.
+    exfalso.
+    unfold exprD in *. destruct (split_env vs).
+    forward.
+    destruct (@e_starOk SSLO _ _ _ _ _ _ H0 H1).
+    intuition; congruence.
+  Qed.
+
+  Lemma exprD_e_empOk
+  : forall us vs,
+    exists val : typD ts nil SL,
+      exprD us vs SSL.(e_emp) SL = Some val /\
+      (val -|- empSP).
+  Proof.
+    unfold exprD; intros; destruct (split_env vs).
+    destruct (SSLO.(e_empOk) us x) as [ ? [ ? ? ] ].
+    rewrite H. eauto.
+  Qed.
+
+  Lemma exprD_e_trueOk
+  : forall us vs,
+    exists val,
+      exprD us vs SSL.(e_true) SL = Some val /\
+      (val -|- ltrue).
+  Proof.
+    unfold exprD; intros; destruct (split_env vs).
+    destruct (SSLO.(e_trueOk) us x) as [ ? [ ? ? ] ].
+    rewrite H. eauto.
+  Qed.
+
+  Lemma exprD_e_starOk
+  : forall us vs x y valx valy,
+      exprD us vs x SL = Some valx ->
+      exprD us vs y SL = Some valy ->
+      exists val,
+        exprD us vs (SSL.(e_star) x y) SL = Some val /\
+        (val -|- valx ** valy).
+  Proof.
+    unfold exprD; intros; destruct (split_env vs).
+    forward.
+    destruct (@e_starOk SSLO us x0 x y _ _ H H0) as [ ? [ ? ? ] ].
+    rewrite H3. inv_all; subst. eauto.
+  Qed.
+
+  Lemma exprD_e_starValid
+  : forall us vs x y val,
+      exprD us vs (SSL.(e_star) x y) SL = Some val ->
+      exists valx valy,
+        exprD us vs x SL = Some valx /\
+        exprD us vs y SL = Some valy /\
+        (val -|- valx ** valy).
+  Proof.
+    unfold exprD; intros; destruct (split_env vs).
+    forward.
+    edestruct (@e_starValid SSLO us x0 x) as [ ? [ ? [ ? [ ? ? ] ] ] ]; eauto.
+    Cases.rewrite_all_goal.
+    inv_all; subst. eauto.
+  Qed.
+
+  Lemma exprD_e_andOk
+  : forall us vs x y valx valy,
+      exprD us vs x SL = Some valx ->
+      exprD us vs y SL = Some valy ->
+      exists val,
+        exprD us vs (SSL.(e_and) x y) SL = Some val /\
+        (val -|- valx //\\ valy).
+  Proof.
+    unfold exprD; intros; destruct (split_env vs).
+    forward.
+    destruct (@e_andOk SSLO us x0 x y _ _ H H0) as [ ? [ ? ? ] ].
+    rewrite H3. inv_all; subst. eauto.
+  Qed.
+
+  Lemma exprD_e_andValid
+  : forall us vs x y val,
+      exprD us vs (SSL.(e_and) x y) SL = Some val ->
+      exists valx valy,
+        exprD us vs x SL = Some valx /\
+        exprD us vs y SL = Some valy /\
+        (val -|- valx //\\ valy).
+  Proof.
+    unfold exprD; intros; destruct (split_env vs).
+    forward.
+    edestruct (@e_andValid SSLO us x0 x) as [ ? [ ? [ ? [ ? ? ] ] ] ]; eauto.
+    Cases.rewrite_all_goal.
+    inv_all; subst. eauto.
   Qed.
 
   Ltac go_crazy :=
@@ -198,10 +352,10 @@ Section syn_sep_log.
         |- _ =>
         destruct (@e_andOk SSLO _ _ _ _ _ _ H H') as [ ? [ ? ? ] ]
       | H : exprD' _ _ _ _ = None |- _ =>
-        first [ erewrite (@e_starOk_None1 _ _ _ _ H) in *
-              | erewrite (@e_starOk_None2 _ _ _ _ H) in *
-              | erewrite (@e_andOk_None1 _ _ _ _ H) in *
-              | erewrite (@e_andOk_None2 _ _ _ _ H) in * ]
+        first [ erewrite (@exprD'_e_starOk_None1 _ _ _ _ H) in *
+              | erewrite (@exprD'_e_starOk_None2 _ _ _ _ H) in *
+              | erewrite (@exprD'_e_andOk_None1 _ _ _ _ H) in *
+              | erewrite (@exprD'_e_andOk_None2 _ _ _ _ H) in * ]
 
       | H : exprD' _ _ _ _ = None |- _ =>
         first [ congruence
@@ -217,7 +371,7 @@ Section syn_sep_log.
   Require Import MirrorCore.Ext.ExprSem.
 
   Lemma Sem_equiv_e_and_assoc
-  : forall a b c : expr sym, forall us vs,
+  :forall us vs, forall a b c : expr sym,
       Sem_equiv _ SL lequiv us vs (SSL.(e_and) a (SSL.(e_and) b c)) (SSL.(e_and) (SSL.(e_and) a b) c).
   Proof.
     clear - IL SSL SSLO. intros.
@@ -251,7 +405,7 @@ Section syn_sep_log.
   Qed.
 
   Lemma Sem_equiv_e_star_assoc
-  : forall a b c : expr sym, forall us vs,
+  : forall us vs, forall a b c : expr sym,
       Sem_equiv _ SL lequiv us vs (SSL.(e_star) a (SSL.(e_star) b c)) (SSL.(e_star) (SSL.(e_star) a b) c).
   Proof.
     clear - IL SSL SSLO BIL. intros.
@@ -289,7 +443,6 @@ Section syn_sep_log.
               Sem_equiv _ SL lequiv us vs ==>
               Sem_equiv _ SL lequiv us vs) SSL.(e_and).
   Proof.
-(*
     unfold Sem_equiv. red. red. red.
     unfold exprD. intros.
     destruct (split_env vs).
@@ -298,10 +451,13 @@ Section syn_sep_log.
         consider X; intros
     end; repeat go_crazy; forward; repeat go_crazy.
     { inv_all; subst.
-      intros. rewrite H3. rewrite H4. rewrite H9.
-      rewrite H5. reflexivity. }
-  Qed. *)
-Admitted.
+      intros.
+      forward.
+      repeat go_crazy.
+      inv_all; subst.
+      Cases.rewrite_all.
+      reflexivity. }
+  Qed.
 
   Lemma Sem_equiv_Proper_e_star
   : forall us vs,
@@ -309,18 +465,19 @@ Admitted.
               Sem_equiv _ SL lequiv us vs ==>
               Sem_equiv _ SL lequiv us vs) SSL.(e_star).
   Proof.
-(*
     unfold Sem_equiv; do 3 red; simpl; intros.
+    unfold exprD in *.
     destruct (split_env vs).
     match goal with
       | |- match ?X with _ => _ end =>
         consider X; intros
     end; repeat go_crazy; forward; repeat go_crazy.
-    { inv_all; subst.
-      intros. rewrite H3. rewrite H4. rewrite H9.
-      rewrite H5. reflexivity. }
-  Qed. *)
-  Admitted.
+    { inv_all; subst. forward.
+      repeat go_crazy.
+      inv_all; subst.
+      Cases.rewrite_all.
+      reflexivity. }
+  Qed.
 
   Lemma ltrue_unitL : forall a, land ltrue a -|- a.
   Proof.
@@ -345,116 +502,109 @@ Admitted.
   Qed.
 
   Lemma Sem_equiv_e_true_e_and_unitLL
-  : forall a : expr sym, forall tus tvs,
+  : forall tus tvs, forall a : expr sym,
       Sem_equiv _ SL lequiv tus tvs (SSL.(e_and) SSL.(e_true) a) a.
   Proof.
-(*
     red; intros.
-    destruct (SSLO.(e_trueOk) (join_env us) tvs) as [ ? [ ? ? ] ].
-    consider (exprD' (join_env us) tvs a SL); intros; repeat go_crazy; auto.
+    unfold exprD. destruct (split_env tvs).
+    destruct (SSLO.(e_trueOk) tus x) as [ ? [ ? ? ] ].
+    consider (exprD' tus x a SL); intros; repeat go_crazy; auto.
     inv_all; subst; intros.
     Cases.rewrite_all_goal. clear - IL.
     rewrite ltrue_unitL. reflexivity.
   Qed.
-*) Admitted.
 
   Lemma Sem_equiv_e_true_e_and_unitLR
-  : forall a : expr sym, forall tus tvs,
+  : forall tus tvs, forall a : expr sym,
       Sem_equiv _ SL lequiv tus tvs (SSL.(e_and) a SSL.(e_true)) a.
   Proof.
-(*
     red; intros.
-    destruct (SSLO.(e_trueOk) (join_env us) tvs) as [ ? [ ? ? ] ].
-    consider (exprD' (join_env us) tvs a SL); intros; repeat go_crazy; auto.
+    unfold exprD. destruct (split_env tvs).
+    destruct (SSLO.(e_trueOk) tus x) as [ ? [ ? ? ] ].
+    consider (exprD' tus x a SL); intros; repeat go_crazy; auto.
     inv_all; subst; intros.
     Cases.rewrite_all. clear - IL.
     rewrite ltrue_unitR. reflexivity.
   Qed.
-*) Admitted.
 
   Lemma Sem_equiv_e_true_e_and_unitRL
-  : forall a : expr sym, forall tus tvs,
+  : forall tus tvs, forall a : expr sym,
       Sem_equiv _ SL lequiv tus tvs a (SSL.(e_and) SSL.(e_true) a).
   Proof.
-(*
     red; intros.
-    destruct (SSLO.(e_trueOk) (join_env us) tvs) as [ ? [ ? ? ] ].
-    consider (exprD' (join_env us) tvs a SL); intros; repeat go_crazy; auto.
+    unfold exprD. destruct (split_env tvs).
+    destruct (SSLO.(e_trueOk) tus x) as [ ? [ ? ? ] ].
+    consider (exprD' tus x a SL); intros; repeat go_crazy; auto.
     inv_all; subst; intros.
     Cases.rewrite_all. clear - IL.
     rewrite ltrue_unitL. reflexivity.
   Qed.
-*) Admitted.
 
   Lemma Sem_equiv_e_true_e_and_unitRR
-  : forall a : expr sym, forall tus tvs,
+  : forall tus tvs, forall a : expr sym,
       Sem_equiv _ SL lequiv tus tvs a (SSL.(e_and) a SSL.(e_true)).
   Proof.
-(*
     red; intros.
-    destruct (SSLO.(e_trueOk) (join_env us) tvs) as [ ? [ ? ? ] ].
-    consider (exprD' (join_env us) tvs a SL); intros; repeat go_crazy; auto.
+    unfold exprD. destruct (split_env tvs).
+    destruct (SSLO.(e_trueOk) tus x) as [ ? [ ? ? ] ].
+    consider (exprD' tus x a SL); intros; repeat go_crazy; auto.
     inv_all; subst; intros.
     Cases.rewrite_all. clear - IL.
     rewrite ltrue_unitR. reflexivity.
   Qed.
-*) Admitted.
+
 
   Lemma Sem_equiv_e_emp_e_star_unitLL
-  : forall a : expr sym, forall tus tvs,
+  : forall tus tvs, forall a : expr sym,
       Sem_equiv _ SL lequiv tus tvs (SSL.(e_star) SSL.(e_emp) a) a.
   Proof.
-(*
     red; intros.
-    destruct (e_empOk SSLO (join_env us) tvs) as [ ? [ ? ? ] ].
-    consider (exprD' (join_env us) tvs a SL); intros; repeat go_crazy; auto.
+    unfold exprD. destruct (split_env tvs).
+    destruct (SSLO.(e_empOk) tus x) as [ ? [ ? ? ] ].
+    consider (exprD' tus x a SL); intros; repeat go_crazy; auto.
     inv_all; subst; intros.
     Cases.rewrite_all. clear - BIL IL.
     rewrite empSPL. reflexivity.
   Qed.
-*) Admitted.
 
   Lemma Sem_equiv_e_emp_e_star_unitLR
-  : forall a : expr sym, forall tus tvs,
+  : forall tus tvs, forall a : expr sym,
       Sem_equiv _ SL lequiv tus tvs (SSL.(e_star) a SSL.(e_emp)) a.
   Proof.
-(*
     red; intros.
-    destruct (SSLO.(e_empOk) (join_env us) tvs) as [ ? [ ? ? ] ].
-    consider (exprD' (join_env us) tvs a SL); intros; repeat go_crazy; auto.
+    unfold exprD. destruct (split_env tvs).
+    destruct (SSLO.(e_empOk) tus x) as [ ? [ ? ? ] ].
+    consider (exprD' tus x a SL); intros; repeat go_crazy; auto.
     inv_all; subst; intros.
-    Cases.rewrite_all. clear - BIL.
+    Cases.rewrite_all. clear - BIL IL.
     rewrite empSPR. reflexivity.
   Qed.
-*) Admitted.
 
   Lemma Sem_equiv_e_emp_e_star_unitRL
-  : forall a : expr sym, forall tus tvs,
+  : forall tus tvs, forall a : expr sym,
       Sem_equiv _ SL lequiv tus tvs a (SSL.(e_star) SSL.(e_emp) a).
   Proof.
-(*
     red; intros.
-    destruct (SSLO.(e_empOk) (join_env us) tvs) as [ ? [ ? ? ] ].
-    consider (exprD' (join_env us) tvs a SL); intros; repeat go_crazy; auto.
+    unfold exprD. destruct (split_env tvs).
+    destruct (SSLO.(e_empOk) tus x) as [ ? [ ? ? ] ].
+    consider (exprD' tus x a SL); intros; repeat go_crazy; auto.
     inv_all; subst; intros.
-    Cases.rewrite_all. clear - BIL.
+    Cases.rewrite_all. clear - BIL IL.
     rewrite empSPL. reflexivity.
   Qed.
-*) Admitted.
 
   Lemma Sem_equiv_e_emp_e_star_unitRR
-  : forall a : expr sym, forall tus tvs,
+  : forall tus tvs, forall a : expr sym,
       Sem_equiv _ SL lequiv tus tvs a (SSL.(e_star) a SSL.(e_emp)).
   Proof.
-(*
     red; intros.
-    destruct (SSLO.(e_empOk) (join_env us) tvs) as [ ? [ ? ? ] ].
-    consider (exprD' (join_env us) tvs a SL); intros; repeat go_crazy; auto.
+    unfold exprD. destruct (split_env tvs).
+    destruct (SSLO.(e_empOk) tus x) as [ ? [ ? ? ] ].
+    consider (exprD' tus x a SL); intros; repeat go_crazy; auto.
     inv_all; subst; intros.
-    Cases.rewrite_all. clear - BIL.
+    Cases.rewrite_all. clear - BIL IL.
     rewrite empSPR. reflexivity.
   Qed.
-*) Admitted.
 
 End syn_sep_log.
 
@@ -488,13 +638,51 @@ Ltac go_crazy SSL SSLO :=
       |- _ ] =>
       destruct (@e_andOk _ _ _ _ _ _ _ SSLO _ _ _ _ _ _ H H') as [ ? [ ? ? ] ]
     | [ H : exprD' _ _ _ _ = None |- _ ] =>
-      first [ erewrite (@e_starOk_None1 _ _ _ _ _ _ _ SSLO _ _ _ _ H) in *
-            | erewrite (@e_starOk_None2 _ _ _ _ _ _ _ SSLO _ _ _ _ H) in *
-            | erewrite (@e_andOk_None1 _ _ _ _ _ _ _ SSLO _ _ _ _ H) in *
-            | erewrite (@e_andOk_None2 _ _ _ _ _ _ _ SSLO _ _ _ _ H) in * ]
-
+      first [ erewrite (@exprD'_e_starOk_None1 _ _ _ _ _ _ _ SSLO _ _ _ _ H) in *
+            | erewrite (@exprD'_e_starOk_None2 _ _ _ _ _ _ _ SSLO _ _ _ _ H) in *
+            | erewrite (@exprD'_e_andOk_None1 _ _ _ _ _ _ _ SSLO _ _ _ _ H) in *
+            | erewrite (@exprD'_e_andOk_None2 _ _ _ _ _ _ _ SSLO _ _ _ _ H) in * ]
     | [ H : exprD' _ _ _ _ = None |- _ ] =>
       first [ congruence
             | apply (@exprD'_e_star_None _ _ _ _ _ _ _ _ SSLO) in H; destruct H; try congruence
             | apply (@exprD'_e_and_None _ _ _ _ _ _ _ _ SSLO) in H; destruct H; try congruence ]
+
+
+    | [ H : exprD _ _ _ _ = _ , H' : _ |- _ ] =>
+      rewrite H in H'
+    | [ H : exprD _ _ _ _ = _ |- _ ] =>
+      rewrite H
+    | [ H : exprD _ _ ?C _ = _
+      , H' : exprD _ _ ?D _ = _
+      |- context [ exprD ?A ?B (SSL.(e_and) ?C ?D) ?T ] ] =>
+      destruct (@exprD_e_andOk _ _ _ _ _ _ _ _ SSLO _ _ _ _ _ _ H H') as [ ? [ ? ? ] ]
+    | [ H : exprD _ _ ?C _ = _
+      , H' : exprD _ _ ?D _ = _
+      |- context [ exprD ?A ?B (SSL.(e_star) ?C ?D) ?T ] ] =>
+      destruct (@exprD_e_starOk _ _ _ _ _ _ _ _ SSLO _ _ _ _ _ _ H H') as [ ? [ ? ? ] ]
+    | [ H : exprD _ _ (SSL.(e_and) _ _) _ = _ |- _ ] =>
+      eapply (@exprD_e_andValid _ _ _ _ _ _ _ _ SSLO) in H ; destruct H as [ ? [ ? [ ? [ ? ? ] ] ] ]
+    | [ H : exprD _ _ (SSL.(e_star) _ _) _ = _ |- _ ] =>
+      eapply (@exprD_e_starValid _ _ _ _ _ _ _ _ SSLO) in H ; destruct H as [ ? [ ? [ ? [ ? ? ] ] ] ]
+    | [ H : exprD _ _ ?C _ = _
+      , H' : exprD _ _ ?D _ = _
+      , H'' : context [ exprD ?A ?B (SSL.(e_star) ?C ?D) ?T ]
+      |- _ ] =>
+      destruct (@exprD_e_starOk _ _ _ _ _ _ _ SSLO _ _ _ _ _ _ H H') as [ ? [ ? ? ] ]
+    | [ H : exprD _ _ ?C _ = _
+      , H' : exprD _ _ ?D _ = _
+      , H'' : context [ exprD ?A ?B (SSL.(e_and) ?C ?D) ?T ]
+      |- _ ] =>
+      destruct (@exprD_e_andOk _ _ _ _ _ _ _ SSLO _ _ _ _ _ _ H H') as [ ? [ ? ? ] ]
+
+    | [ H : exprD _ _ _ _ = None |- _ ] =>
+      first [ erewrite (@exprD_e_starOk_None1 _ _ _ _ _ _ _ SSLO _ _ _ _ H) in *
+            | erewrite (@exprD_e_starOk_None2 _ _ _ _ _ _ _ SSLO _ _ _ _ H) in *
+            | erewrite (@exprD_e_andOk_None1 _ _ _ _ _ _ _ SSLO _ _ _ _ H) in *
+            | erewrite (@exprD_e_andOk_None2 _ _ _ _ _ _ _ SSLO _ _ _ _ H) in * ]
+
+    | [ H : exprD _ _ _ _ = None |- _ ] =>
+      first [ congruence
+            | apply (@exprD_e_star_None _ _ _ _ _ _ _ _ SSLO) in H; destruct H; try congruence
+            | apply (@exprD_e_and_None _ _ _ _ _ _ _ _ SSLO) in H; destruct H; try congruence ]
   end.
